eve/Src/framework/eiffel2boogie/translation/custom/e2b_custom_ownership_handler.e
@@ -1,0 +1,47 @@
+note
+	description: "Summary description for {E2B_CUSTOM_OWNERSHIP_HANDLER}."
+	date: "$Date$"
+	revision: "$Revision$"
+
+class
+	E2B_CUSTOM_OWNERSHIP_HANDLER
+
+inherit
+
+	E2B_CUSTOM_CALL_HANDLER
+
+	SHARED_WORKBENCH
+
+feature -- Status report
+
+	is_handling_call (a_target_type: TYPE_A; a_feature: FEATURE_I): BOOLEAN
+			-- <Precursor>
+		do
+			Result :=
+				a_feature.written_in = system.any_id and then
+				a_feature.feature_name.ends_with ("_")
+		end
+
+feature -- Basic operations
+
+	handle_routine_call_in_body (a_translator: E2B_BODY_EXPRESSION_TRANSLATOR; a_feature: FEATURE_I; a_parameters: BYTE_LIST [PARAMETER_B])
+			-- <Precursor>
+		local
+			l_name: STRING
+			l_parameters: BYTE_LIST [PARAMETER_B]
+		do
+
+			l_name := a_feature.feature_name.substring (1, a_feature.feature_name.count-1)
+			if l_name ~ "wrap" or l_name ~ "unwrap" then
+
+			else
+				a_translator.process_builtin_routine_call (a_feature, a_parameters, l_name)
+			end
+		end
+
+	handle_routine_call_in_contract (a_translator: E2B_CONTRACT_EXPRESSION_TRANSLATOR; a_feature: FEATURE_I; a_parameters: BYTE_LIST [PARAMETER_B])
+			-- <Precursor>
+		do
+		end
+
+end
